qcp/ast/VC/subst_proof_manual.v
@@ -21,31 +21,33 @@ From SimpleC.EE Require Import malloc.
 From SimpleC.EE Require Import sll_tmpl.
 Local Open Scope sac.
 
-Lemma proof_of_subst_var_return_wit_1_1 : subst_var_return_wit_1_1.
-Proof. Admitted. 
+Lemma proof_of_subst_var_safety_wit_5 : subst_var_safety_wit_5.
+Proof. 
+    pre_process.
+    Admitted. 
 
-Lemma proof_of_subst_var_return_wit_1_2 : subst_var_return_wit_1_2.
-Proof.
+Lemma proof_of_subst_var_return_wit_1_1 : subst_var_return_wit_1_1.
+Proof.    
     pre_process.
     unfold list_Z_cmp in H0.
     rewrite H in H0.
     destruct (list_Z_eqb qvar src_str) eqn:Heq; [ | discriminate ].
     unfold term_subst_v.
-    rewrite H1, Heq.
+    rewrite H2, Heq.
     unfold store_term at 2.
     simpl.
     fold store_term.
     Exists y z. 
     entailer!.
-Qed. 
+Qed.  
 
-Lemma proof_of_subst_var_return_wit_1_3 : subst_var_return_wit_1_3.
-Proof.
+Lemma proof_of_subst_var_return_wit_1_2 : subst_var_return_wit_1_2.
+Proof. 
     pre_process.
     unfold list_Z_cmp in H1.
     destruct (list_Z_eqb qvar src_str) eqn:Heq; [ contradiction | ].
     unfold term_subst_v.
-    rewrite H2, Heq.
+    rewrite H3, Heq.
     fold term_subst_v.
     unfold store_term at 2.
     simpl.
@@ -53,13 +55,13 @@ Proof.
     Exists y z.
     rewrite H.
     entailer!.
-Qed. 
+Qed.
 
-Lemma proof_of_subst_var_return_wit_1_4 : subst_var_return_wit_1_4.
-Proof.
+Lemma proof_of_subst_var_return_wit_1_3 : subst_var_return_wit_1_3.
+Proof. 
     pre_process.
     unfold term_subst_v at 3.
-    rewrite H1.
+    rewrite H2.
     fold term_subst_v.
     unfold store_term at 3.
     simpl.
@@ -67,37 +69,37 @@ Proof.
     Exists y z.
     rewrite H, H0.
     entailer!.
-Qed.
+Qed. 
+
+Lemma proof_of_subst_var_return_wit_1_4 : subst_var_return_wit_1_4.
+Proof.
+    pre_process.
+    unfold term_subst_v.
+    rewrite H0.
+    unfold store_term.
+    entailer!.
+Qed. 
 
 Lemma proof_of_subst_var_return_wit_1_5 : subst_var_return_wit_1_5.
 Proof. 
     pre_process.
+    unfold list_Z_cmp in H0.
+    destruct (list_Z_eqb var src_str) eqn:Heq; [ contradiction | ].
     unfold term_subst_v.
-    rewrite H.
+    rewrite H2, Heq.
     unfold store_term.
+    Exists y.
     entailer!.
 Qed.
 
 Lemma proof_of_subst_var_return_wit_1_6 : subst_var_return_wit_1_6.
 Proof.
     pre_process.
-    unfold list_Z_cmp in H0.
-    destruct (list_Z_eqb var src_str) eqn:Heq; [ contradiction | ].
-    unfold term_subst_v.
-    rewrite H1, Heq.
-    unfold store_term.
-    Exists y.
-    entailer!.
-Qed.
-    
-Lemma proof_of_subst_var_return_wit_1_7 : subst_var_return_wit_1_7.
-Proof. 
-    pre_process.
     unfold list_Z_cmp in H1.
     rewrite H0 in H1.
     destruct (list_Z_eqb var src_str) eqn:Heq; [ | discriminate ].
     unfold term_subst_v.
-    rewrite H2, Heq.
+    rewrite H3, Heq.
     unfold store_term.
     Exists retval.
     entailer!.
@@ -107,22 +109,36 @@ Lemma proof_of_subst_var_partial_solve_wit_4_pure : subst_var_partial_solve_wit_
 Proof.
     pre_process.
     unfold store_string.
-    entailer!. 
+    Intros n1 n2 n3.
+    entailer!.
+Qed.
     
-    Admitted. 
-
 Lemma proof_of_subst_var_partial_solve_wit_8_pure : subst_var_partial_solve_wit_8_pure.
 Proof. 
-    pre_process. Admitted. 
+    pre_process.
+    unfold store_string.
+    Intros n1 n2.
+    sep_apply store_term_unfold.
+    entailer!.
+Qed.
 
 Lemma proof_of_subst_var_partial_solve_wit_9_pure : subst_var_partial_solve_wit_9_pure.
 Proof.
-    pre_process. Admitted. 
-
+    pre_process.
+    unfold store_string.
+    Intros n1 n2.
+    sep_apply store_term_unfold.
+    entailer!.
+Qed.
+    
 Lemma proof_of_subst_var_partial_solve_wit_12_pure : subst_var_partial_solve_wit_12_pure.
 Proof.
     pre_process.
-    entailer!. Admitted. 
+    unfold store_string.
+    Intros n1 n2 n3.
+    sep_apply (store_term_unfold z qterm).
+    entailer!.
+Qed.
 
 Lemma proof_of_subst_var_which_implies_wit_1 : subst_var_which_implies_wit_1.
 Proof. 
@@ -134,7 +150,7 @@ Qed.
 Lemma proof_of_subst_var_which_implies_wit_2 : subst_var_which_implies_wit_2.
 Proof.
     pre_process.
-    sep_apply store_term'_Var; [ | tauto].
+    sep_apply store_term'_Var; [ | tauto | tauto].
     Intros var y.
     Exists y var.
     entailer!.
@@ -143,7 +159,7 @@ Qed.
 Lemma proof_of_subst_var_which_implies_wit_3 : subst_var_which_implies_wit_3.
 Proof. 
     pre_process.
-    sep_apply store_term'_Const; [ | tauto].
+    sep_apply store_term'_Const; [ | tauto | tauto].
     Intros y z.
     Exists y z.
     entailer!.
@@ -152,7 +168,7 @@ Qed.
 Lemma proof_of_subst_var_which_implies_wit_4 : subst_var_which_implies_wit_4.
 Proof. 
     pre_process.
-    sep_apply store_term'_Apply; [ | tauto].
+    sep_apply store_term'_Apply; [ | tauto | tauto].
     Intros lt rt y z.
     Exists z y lt rt.
     entailer!.
@@ -161,38 +177,36 @@ Qed.
 Lemma proof_of_subst_var_which_implies_wit_5 : subst_var_which_implies_wit_5.
 Proof. 
     pre_process.
-    sep_apply store_term'_Quant; [ | tauto].
+    sep_apply store_term'_Quant; [ | tauto | tauto].
     Intros typ v b y z.
     Exists z y typ v b.
     entailer!.
 Qed. 
 
+Lemma proof_of_subst_term_safety_wit_5 : subst_term_safety_wit_5.
+Proof. Admitted. 
+
 Lemma proof_of_subst_term_return_wit_1_1 : subst_term_return_wit_1_1.
 Proof. 
-    pre_process.
-    Admitted.
-
-Lemma proof_of_subst_term_return_wit_1_2 : subst_term_return_wit_1_2.
-Proof.
     pre_process.
     unfold list_Z_cmp in H0.
     rewrite H in H0.
     destruct (list_Z_eqb qvar src_str) eqn:Heq; [ | discriminate ].
     unfold term_subst_t.
-    rewrite H1, Heq.
+    rewrite H2, Heq.
     unfold store_term at 3.
     fold store_term.
     Exists y z. 
     entailer!.
 Qed.
-    
-Lemma proof_of_subst_term_return_wit_1_3 : subst_term_return_wit_1_3.
-Proof. 
+
+Lemma proof_of_subst_term_return_wit_1_2 : subst_term_return_wit_1_2.
+Proof.  
     pre_process.
     unfold list_Z_cmp in H0.
     destruct (list_Z_eqb qvar src_str) eqn:Heq; [ contradiction | ].
     unfold term_subst_t.
-    rewrite H1, Heq.
+    rewrite H2, Heq.
     fold term_subst_t.
     unfold store_term at 3.
     fold store_term.
@@ -200,11 +214,11 @@ Proof.
     entailer!.
 Qed.
 
-Lemma proof_of_subst_term_return_wit_1_4 : subst_term_return_wit_1_4.
+Lemma proof_of_subst_term_return_wit_1_3 : subst_term_return_wit_1_3.
 Proof. 
     pre_process.
     unfold term_subst_t at 3.
-    rewrite H.
+    rewrite H0.
     fold term_subst_t.
     unfold store_term at 4.
     fold store_term.
@@ -212,16 +226,16 @@ Proof.
     entailer!.
 Qed.
 
-Lemma proof_of_subst_term_return_wit_1_5 : subst_term_return_wit_1_5.
-Proof. 
+Lemma proof_of_subst_term_return_wit_1_4 : subst_term_return_wit_1_4.
+Proof.  
     pre_process.
     unfold term_subst_t.
-    rewrite H.
+    rewrite H0.
     unfold store_term at 2.
     entailer!.
 Qed.
 
-Lemma proof_of_subst_term_return_wit_1_6 : subst_term_return_wit_1_6.
+Lemma proof_of_subst_term_return_wit_1_5 : subst_term_return_wit_1_5.
 Proof. 
     pre_process.
     unfold list_Z_cmp in H0.
@@ -233,7 +247,7 @@ Proof.
     entailer!.
 Qed.
 
-Lemma proof_of_subst_term_return_wit_1_7 : subst_term_return_wit_1_7.
+Lemma proof_of_subst_term_return_wit_1_6 : subst_term_return_wit_1_6.
 Proof. 
     pre_process.
     unfold list_Z_cmp in H1.
@@ -245,13 +259,31 @@ Proof.
 Qed.
 
 Lemma proof_of_subst_term_partial_solve_wit_9_pure : subst_term_partial_solve_wit_9_pure.
-Proof. Admitted. 
+Proof.
+    pre_process.
+    unfold store_string.
+    Intros n.
+    sep_apply (store_term_unfold y lt).
+    entailer!.
+Qed.
 
 Lemma proof_of_subst_term_partial_solve_wit_10_pure : subst_term_partial_solve_wit_10_pure.
-Proof. Admitted. 
+Proof. 
+    pre_process.
+    unfold store_string.
+    Intros n.
+    sep_apply (store_term_unfold z rt).
+    entailer!.
+Qed. 
 
 Lemma proof_of_subst_term_partial_solve_wit_13_pure : subst_term_partial_solve_wit_13_pure.
-Proof. Admitted. 
+Proof.
+    pre_process.
+    unfold store_string.
+    Intros n1 n2.
+    sep_apply (store_term_unfold z qterm).
+    entailer!.
+Qed. 
 
 Lemma proof_of_subst_term_which_implies_wit_1 : subst_term_which_implies_wit_1.
 Proof. 
@@ -263,7 +295,7 @@ Qed.
 Lemma proof_of_subst_term_which_implies_wit_2 : subst_term_which_implies_wit_2.
 Proof. 
     pre_process.
-    sep_apply store_term'_Var; [ | tauto].
+    sep_apply store_term'_Var; [ | tauto | tauto].
     Intros var y.
     Exists y var.
     entailer!.
@@ -281,7 +313,7 @@ Qed.
 Lemma proof_of_subst_term_which_implies_wit_4 : subst_term_which_implies_wit_4.
 Proof.
     pre_process.
-    sep_apply store_term'_Const; [ | tauto].
+    sep_apply store_term'_Const; [ | tauto | tauto].
     Intros y z.
     Exists y z.
     entailer!.
@@ -290,7 +322,7 @@ Qed.
 Lemma proof_of_subst_term_which_implies_wit_5 : subst_term_which_implies_wit_5.
 Proof. 
     pre_process.
-    sep_apply store_term'_Apply; [ | tauto].
+    sep_apply store_term'_Apply; [ | tauto | tauto].
     Intros lt rt y z.
     Exists z y lt rt.
     entailer!.
@@ -299,7 +331,7 @@ Qed.
 Lemma proof_of_subst_term_which_implies_wit_6 : subst_term_which_implies_wit_6.
 Proof. 
     pre_process.
-    sep_apply store_term'_Quant; [ | tauto].
+    sep_apply store_term'_Quant; [ | tauto | tauto].
     Intros typ v b y z.
     Exists z y typ v b.
     entailer!.
